New approach with a restricted version of simulations: no restrict clause and removed sm_inject_separated.

core/effect_simulations_trans2.v
@@ -15,12 +15,20 @@ Require Import core_semantics_lemmas.
 Require Import StructuredInjections.
 Require Import reach.
 Require Import effect_semantics.
-Require Import effect_simulations.
+(*Load effect_simulations2.*)
+(*Load no_junk.*)
+(*Require Import effect_simulations.*)
+Require Import effect_simulations2.
 Require Import effect_simulations_lemmas.
 Require Import Wellfounded.
 Require Import Relations.
-Require Import effect_corediagram_trans.
+Require Import effect_corediagram_trans2.
+(*Require Import effect_corediagram_trans.*)
 Require Import effect_interpolants.
+Require Import mem_interpolation_defs.
+
+Require Import pure.
+Require Import full_composition.
 
 Declare Module EFFAX : EffectInterpolationAxioms.
 
@@ -68,7 +76,7 @@ Lemma initial_inject_split: forall j m1 m3 (Inj:Mem.inject j m1 m3),
                (exists m : positive,
                    b2 = (Mem.nextblock Mem.empty + m)%positive /\
                    compose_meminj j1 j2 (Mem.nextblock Mem.empty + m)%positive =
-                   Some (b3, ofs3))).
+                   Some (b3, ofs3))) /\ pure_composition j1 j2 m1 m2.
 Proof. intros.
   destruct (EFFAX.interpolate_II_strongHeqMKI _ _ _ 
      empty_inj _ (empty_fwd m1) _ _ empty_inj _ (empty_fwd m3) _ Inj)
@@ -87,7 +95,7 @@ subst. exists m2, j1, j2.
 split; trivial.
 split; trivial.
 split; trivial.
-destruct AA as [_ [_ [_ [_ [_ [XX YY]]]]]].
+destruct AA as [_ [Pure [_ [_ [XX YY]]]]].
 split. intros.
   split; intros. destruct H as [b3 [d COMP]].
     destruct (compose_meminjD_Some _ _ _ _ _ COMP) as
@@ -107,7 +115,7 @@ split. intros.
       destruct AA as [? [? ?]]; subst. intuition.
     destruct AA as [? [? ?]]; subst. intuition.
     destruct AA as [mm [[? ?] ?]]; subst. intuition.
-apply YY.
+split; auto.
 Qed.
 
 Lemma compose_sm_sharedSrc mu12 mu23: forall
@@ -182,11 +190,6 @@ Context {F1 V1 C1 F2 V2 C2 F3 V3 C3:Type}
         (g2 : Genv.t F2 V2)
         (g3 : Genv.t F3 V3).
 
-Definition I_fiddle (mu12 mu23:SM_Injection): Prop :=
-  forall b2 delta23, extern_of mu23 b2 = Some (b3, delta23) ->
-          forall ofs, 
-            Mem.perm m2 b2 ofs Max NE ->
-            source mu12 m1 b2 ofs = Some (b1, delta12).
 
 Theorem eff_sim_trans: forall 
         (SIM12: @SM_simulation_inject _ _ _ _ _ _ Sem1 Sem2 g1 g2)
@@ -197,26 +200,27 @@ Proof. (*follows structure of forward_simulations_trans.injinj*)
   destruct SIM12 
     as [core_data12 match_core12 core_ord12 core_ord_wf12 
       match_sm_wd12 genvs_dom_eq12 match_genv12
-      match_visible12 match_restrict12 
+      match_visible12 (*match_junk_inv12 match_restrict12 *)
       match_sm_valid12 core_initial12 effcore_diagram12
       core_halted12 core_at_external12 eff_after_external12].  
   destruct SIM23 
     as [core_data23 match_core23 core_ord23 core_ord_wf23 
       match_sm_wd23 genvs_dom_eq23 match_genv23
-      match_visible23 match_restrict23
+      match_visible23 (*match_junk_inv23 match_restrict23*)
       match_sm_valid23 core_initial23 effcore_diagram23
       core_halted23 core_at_external23 eff_after_external23].
   eapply Build_SM_simulation_inject with
     (core_ord := clos_trans _ (sem_compose_ord_eq_eq core_ord12 core_ord23 C2))
     (match_state := fun d mu c1 m1 c3 m3 => 
       match d with (d1,X,d2) => 
-        exists c2, exists m2, exists mu1, exists mu2, 
+        exists c2, exists m2, exists mu1, exists mu2,                                 
           X=Some c2 /\ mu = compose_sm mu1 mu2 /\
           (locBlocksTgt mu1 = locBlocksSrc mu2 /\
            extBlocksTgt mu1 = extBlocksSrc mu2 /\
            (forall b, pubBlocksTgt mu1 b = true -> pubBlocksSrc mu2 b = true) /\
            (forall b, frgnBlocksTgt mu1 b = true -> frgnBlocksSrc mu2 b = true)) /\ 
-          match_core12 d1 mu1 c1 m1 c2 m2 /\ match_core23 d2 mu2 c2 m2 c3 m3 
+          match_core12 d1 mu1 c1 m1 c2 m2 /\ match_core23 d2 mu2 c2 m2 c3 m3 /\
+          pure_comp_ext mu1 mu2 m1 m2 /\ full_ext mu1 mu2
       end).
 { (*well_founded*)
   eapply wf_clos_trans. 
@@ -224,7 +228,7 @@ Proof. (*follows structure of forward_simulations_trans.injinj*)
 { (*match_sm_wd*) clear - match_sm_wd12 match_sm_wd23.
   intros. rename c2 into c3. rename m2 into m3.
   destruct d as [[d12 cc2] d23].
-  destruct H as [c2 [m2 [mu12 [mu23 [X [J [INV [MC12 MC23]]]]]]]]; subst.
+  destruct H as [c2 [m2 [mu12 [mu23 [X [J [INV [MC12 [MC23 IFDL]]]]]]]]]; subst.
   specialize (match_sm_wd12 _ _ _ _ _ _ MC12).
   specialize (match_sm_wd23 _ _ _ _ _ _ MC23).
   destruct INV as [INVa [INVb [INVc INVd]]].
@@ -235,7 +239,7 @@ Proof. (*follows structure of forward_simulations_trans.injinj*)
   clear - genvs_dom_eq12 match_sm_wd12 match_genv12 match_genv23.
   intros. rename c2 into c3. rename m2 into m3.
   destruct d as [[d12 cc2] d23].
-  destruct MC as [c2 [m2 [mu12 [mu23 [X [J [INV [MC12 MC23]]]]]]]]; subst.
+  destruct MC as [c2 [m2 [mu12 [mu23 [X [J [INV [MC12 [MC23 IFDL]]]]]]]]]; subst.
   destruct (match_genv12 _ _ _ _ _ _ MC12) as [GE12a GE12b].
   destruct (match_genv23 _ _ _ _ _ _ MC23) as [GE23a GE23b].
   split. apply meminj_preserves_genv2blocks.
@@ -248,20 +252,87 @@ Proof. (*follows structure of forward_simulations_trans.injinj*)
     clear - match_sm_wd12 match_visible12.
     intros. rename c2 into c3. rename m2 into m3.
     destruct d as [[d12 cc2] d23].
-    destruct H as [c2 [m2 [mu12 [mu23 [X [J [INV [MC12 MC23]]]]]]]]; subst.
+    destruct H as [c2 [m2 [mu12 [mu23 [X [J [INV [MC12 [MC23 IFDL]]]]]]]]]; subst.
     simpl. rewrite vis_compose_sm. eapply match_visible12. eassumption. }
-{ (*match_restrict*)
-    clear - match_restrict12.
+(*
+{ (*match_restrict'*)
+  clear - match_restrict12 match_restrict23 match_visible12 match_visible23.
     intros. rename c2 into c3. rename m2 into m3.
     destruct d as [[d12 cc2] d23].
-    destruct H as [c2 [m2 [mu12 [mu23 [XX [J [INV [MC12 MC23]]]]]]]]; 
+    destruct H as [c2 [m2 [mu12 [mu23 [XX [J [INV [MC12 [MC23 pure]]]]]]]]];
+      subst; simpl.
+    (* destruct (ex_clean_mem (restrict_sm mu12 X) m1 m2) as [m2' [JINV NJNK]].
+    remember (clean (restrict_sm mu12 X) m1' m2) as m2'.*)
+    remember (fun b => image mu12 X b || vis mu23 b) as X'.
+    exists c2, m2, (restrict_sm mu12 X), (restrict_sm mu23 X').
+    intuition. 
+    unfold compose_sm; f_equal; 
+    try (solve [unfold restrict_sm; destruct mu12, mu23; simpl; auto]).
+    { rewrite restrict_compose, restrict_sm_local.
+      extensionality b.
+      unfold compose_meminj, restrict.
+      destruct (X b) 
+eqn: Xb; auto.
+      destruct (local_of mu12 b) eqn:imgloc12; try destruct p; auto.
+      cut (local_of mu23 b0 = local_of (restrict_sm mu23 X') b0).
+      + intros HH; rewrite HH; auto.
+      + assert (SMWD:SM_wd mu23) by ad_it .
+        destruct mu23; unfold  restrict_sm, restrict; simpl.
+        destruct (X' b0) eqn:X'b0; auto. 
+        destruct (local_of b0) eqn:locb0; auto.
+        subst X'; simpl in X'b0.  
+        destruct p.
+        apply SMWD in locb0; destruct locb0 as [HH HHH]; simpl in *.
+        unfold vis in X'b0; simpl in X'b0.
+        rewrite HH in X'b0; rewrite orb_true_r in X'b0; inversion X'b0. }
+        { rewrite restrict_compose, restrict_sm_extern.
+          extensionality b.
+          unfold compose_meminj, restrict.
+          destruct (X b) eqn: Xb; auto.
+          destruct (extern_of mu12 b) eqn:imgloc12; try destruct p; auto.
+          cut (extern_of mu23 b0 = extern_of (restrict_sm mu23 X') b0).
+      + intros HH; rewrite HH; auto.
+      + eapply (image_forward
+ mu12 X) in Xb.
+        subst X'.
+        destruct mu23; unfold  restrict_sm, restrict; simpl.
+        rewrite Xb; simpl; auto.
+        instantiate (1:=z).
+        rewrite <- imgloc12.
+        ad_it.
+        }
+    solve [unfold restrict_sm; destruct mu12, mu23; simpl; auto].
+    solve [unfold restrict_sm; destruct mu12, mu23; simpl; auto].
+    solve [unfold restrict_sm; destruct mu12, mu23; simpl; auto].
+    solve [unfold restrict_sm; destruct mu12, mu23; simpl; auto].
+    eapply match_restrict23; eauto.
+    rewrite vis_compose_sm in H0.
+    { intros. subst X'. destruct (vis mu23 b) eqn: visb.
+      + rewrite orb_true_r; auto.
+      + unfold vis in H4. inversion H4. }
+    subst X'. apply REACH_closed_union.
+    ad_it. (* REACH_closed m2 (image mu12 X) *)
+    eapply (match_visible23 _ _ _ _ _ _ MC23).
+    ad_it. }
+{ (*match_restrict*)
+  clear - match_restrict12 match_restrict23 match_junk_inv12 match_junk_inv23.
+    intros. rename c2 into c3. rename m2 into m3.
+    destruct d as [[d12 cc2] d23].
+    destruct H as [c2 [m2 [mu12 [mu23 [XX [J [INV [MC12 [MC23 IFDL]]]]]]]]]; 
       subst; simpl in *.
-    exists c2, m2, (restrict_sm mu12 X), mu23.
+    destruct (ex_clean_mem (restrict_sm mu12 X) m1 m2) as [m2' [JINV NJNK]].
+    exists c2, m2', (restrict_sm mu12 X), (restrict_sm mu12 X).
+    assert (vis' : forall b : block, vis mu23 b = true -> X b = true).
+    generalize H0; clear.
+    unfold compose_sm; unfold vis; simpl; intros.
+    apply H0.
     specialize (match_restrict12 _ _ _ _ _ _ X MC12 H0 H1).
+    specialize (match_restrict23 _ _ _ _ _ _ X MC23 H0 H1).
     intuition.
+    (*apply restrict_sm_WD; eauto.*)
     unfold compose_sm; simpl.
-    f_equal; try (destruct mu12; reflexivity).
-      destruct mu12; simpl in *.
+    f_equal; try (destruct mu12, mu23; reflexivity).
+      destruct mu12, mu23; simpl in *.
         unfold compose_meminj, restrict. extensionality b.
         remember (X b) as d.
         destruct d; trivial.
@@ -272,24 +343,36 @@ Proof. (*follows structure of forward_simulations_trans.injinj*)
       destruct mu12; simpl in *. assumption.
       destruct mu12; simpl in *. assumption.
       destruct mu12; simpl in *. apply (H2 _ H4).
-      destruct mu12; simpl in *. apply (H5 _ H4). }
+      destruct mu12; simpl in *. apply (H5 _ H4).
+
+      apply (match_junk_inv12 _ _ _ _ _ m2); eauto.
+      
+      ad_it.
+
+      move IFDL at bottom.
+      unfold I_fiddle in *. intros b2 ofs perm ext.
+      specialize (IFDL b2 delta23 b3 extern_maps ofs allocated); 
+        destruct IFDL as [b1 [delta12 has_source]].
+      unfold source, sourceN.
+      exists b1, delta12.
+} *) 
 { (*sm_valid*)
     clear - match_sm_valid12 match_sm_valid23.
     intros. rename c2 into c3.  rename m2 into m3.
     destruct d as [[d12 cc2] d23].
-    destruct H as [c2 [m2 [mu12 [mu23 [X [J [INV [MC12 MC23]]]]]]]]; subst.
+    destruct H as [c2 [m2 [mu12 [mu23 [X [J [INV [MC12 [MC23 IFDL]]]]]]]]]; subst.
     specialize (match_sm_valid12 _ _ _ _ _ _ MC12).
     specialize (match_sm_valid23 _ _ _ _ _ _ MC23).
     unfold sm_valid, compose_sm. destruct mu12; destruct mu23; simpl in *.
     split; intros. eapply match_sm_valid12. apply H.
     eapply match_sm_valid23. apply H. }
 { (*initial_core*)
-   clear - genvs_dom_eq12 core_initial12 genvs_dom_eq23 core_initial23.
+  clear - genvs_dom_eq12 core_initial12 genvs_dom_eq23 core_initial23.
    intros. rename m2 into m3. rename v into v3. rename vals2 into vals3. 
     (*assert (HT: Forall2 Val.has_type vals1 (sig_args sig)). 
       eapply forall_valinject_hastype; eassumption.*)
     destruct (initial_inject_split _ _ _ H0) 
-       as [m2 [j1 [j2 [J [Inj12 [Inj23 [X [Y [XX YY]]]]]]]]].
+       as [m2 [j1 [j2 [J [Inj12 [Inj23 [X [Y [XX [YY Pure]]]]]]]]]].
     subst.
     destruct (forall_val_inject_split _ _ _ _ H1)
        as [vals2 [ValsInj12 ValsInj23]].
@@ -403,23 +486,44 @@ Proof. (*follows structure of forward_simulations_trans.injinj*)
   exists c3. 
   split; trivial. 
   exists c2, m2, mu1, mu2.
-  split; trivial.
+  split. auto.
   split. subst. unfold initial_SM, compose_sm; simpl.
            f_equal.
   split. subst; simpl. repeat (split; trivial).
-  split; trivial. }
+  split; trivial.
+  split; trivial.
+  subst.
+  split.
+  
+  (* PURE *)
+  { unfold pure_comp_ext, pure_composition, pure_composition_locat, pure_composition_block, initial_SM; simpl. apply Pure.
+  }
+  
+  (* FULL *)
+  { unfold full_ext, full_comp, initial_SM; simpl.
+    intros. move X at bottom. 
+    assert (H7':exists (b2 : block) (d1 : Z), j1 b0 = Some (b2, d1)) by (exists b1, delta1; auto).
+    apply X in H7'.
+    destruct H7' as [b2 [delta2 HH]].
+    clear - HH H7.
+    unfold compose_meminj in HH; rewrite H7 in HH; simpl.
+    destruct (j2 b1) eqn:result2.
+    destruct p as [b2' delta2']; exists b2', delta2'; auto.
+    inversion HH.
+  }
+ }
 { (*effcore_diagram*)
    clear - match_sm_wd12 match_sm_valid12 effcore_diagram12 
             match_sm_wd23 match_sm_valid23 effcore_diagram23.
    intros. rename st2 into st3. rename m2 into m3.
    destruct cd as [[d12 cc2] d23].
-   destruct H0 as [c2 [m2 [mu12 [mu23 [X [J [INV [MC12 MC23]]]]]]]]; subst.
+   destruct H0 as [c2 [m2 [mu12 [mu23 [X [J [INV [MC12 [MC23 [pure full]]]]]]]]]]; subst.
    eapply effcore_diagram_trans; eassumption. }
 { (*halted*)
   clear - match_sm_wd12 core_halted12 match_sm_wd23 core_halted23.
   intros. rename c2 into c3. rename m2 into m3.  
   destruct cd as [[d12 cc2] d23].
-  destruct H as [c2 [m2 [mu12 [mu23 [X [J [INV [MC12 MC23]]]]]]]]; subst.
+  destruct H as [c2 [m2 [mu12 [mu23 [X [J [INV [MC12 [MC23 [pure full]]]]]]]]]]; subst.
   destruct (core_halted12 _ _ _ _ _ _ _ MC12 H0) as
      [v2 [MInj12 [RValsInject12 HaltedMid]]]. 
   destruct (core_halted23 _ _ _ _ _ _ _ MC23 HaltedMid) as
@@ -441,7 +545,7 @@ Proof. (*follows structure of forward_simulations_trans.injinj*)
   intros. rename c2 into c3. rename m2 into m3.
   rename H0 into AtExtSrc. 
   destruct cd as [[d12 cc2] d23]. 
-  destruct H as [st2 [m2 [mu12 [mu23 [Hst2 [HMu [GLUEINV [MC12 MC23]]]]]]]]. 
+  destruct H as [st2 [m2 [mu12 [mu23 [Hst2 [HMu [GLUEINV [MC12 [MC23 [pure full]]]]]]]]]]. 
   subst.
   destruct (core_at_external12 _ _ _ _ _ _ _ _ _ MC12 AtExtSrc)
     as [MInj12 [vals2 [ArgsInj12 [AtExt2 SH12]]]]; 
@@ -491,7 +595,21 @@ Proof. (*follows structure of forward_simulations_trans.injinj*)
                      intros. do 2 (rewrite orb_true_iff in H1).
                              destruct H1. rewrite H1; trivial.
                              destruct H1. apply GlueF in H1. intuition. apply GlueP in H1. intuition. eauto.
-            rewrite HNU. rewrite compose_sm_shared.
+        (* PURE HERE *)
+        { clear - pure.
+          unfold pure_comp_ext, pure_composition, pure_composition_locat, 
+          pure_composition_block, replace_locals in *;
+          destruct mu12, mu23; simpl in *.
+          apply pure.
+        }
+        (* Full here *)
+        { unfold full_ext, full_comp, replace_locals; simpl.
+          destruct mu12; destruct mu23; simpl.
+          exact full.
+        }
+
+
+        rewrite HNU. rewrite compose_sm_shared.
               eapply Mem.inject_compose; eassumption.
             rewrite replace_locals_pubBlocksTgt, replace_locals_pubBlocksSrc. 
               intros. rewrite GlueL in H. apply andb_true_iff in H. destruct H. 
@@ -526,19 +644,19 @@ Proof. (*follows structure of forward_simulations_trans.injinj*)
   eapply GLUEINV. }
 { (*after_external*)
   clear - match_sm_wd12 match_sm_valid12 core_at_external12 
-          eff_after_external12  match_visible12 match_restrict12
+          eff_after_external12  match_visible12 (*match_restrict12*)
           match_sm_wd23 match_sm_valid23 core_at_external23 
           eff_after_external23.
   intros. rename st2 into st3. rename m2 into m3. 
           rename vals2 into vals3'. rename m2' into m3'.
           rename UnchLOOR into UnchLOOR13.
   destruct cd as [[d12 cc2] d23].
-  destruct MatchMu as [st2 [m2 [mu12 [mu23 [Hst2 [HMu [GLUEINV [MC12 MC23]]]]]]]].
+  destruct MatchMu as [st2 [m2 [mu12 [mu23 [Hst2 [HMu [GLUEINV [MC12 [MC23 [pure full]]]]]]]]]].
   assert (WDmu12:= match_sm_wd12 _ _ _ _ _ _ MC12).
   assert (WDmu23:= match_sm_wd23 _ _ _ _ _ _ MC23).
-  remember (fun b => locBlocksSrc mu12 b || frgnBlocksSrc mu12 b || mapped (as_inj (compose_sm mu12 mu23)) b)
-      as RESTR.
-  assert (NormMC12: match_core12 d12 (restrict_sm mu12 RESTR) st1 m1 st2 m2).
+  remember (fun b => locBlocksSrc mu12 b || frgnBlocksSrc mu12 b || mapped (as_inj (compose_sm mu12 mu23)) b ) as RESTR.
+  assert (NormMC12: match_core12 d12 mu12 st1 m1 st2 m2) by assumption.
+  (*assert (NormMC12: match_core12 d12 (restrict_sm mu12 RESTR) st1 m1 st2 m2).
      apply match_restrict12. apply MC12.
      subst RESTR. clear. intuition.
      subst RESTR.
@@ -548,11 +666,15 @@ Proof. (*follows structure of forward_simulations_trans.injinj*)
               pubTgtHyp pubTgt' pubSrcHyp pubSrc' ValInjMu AtExtTgt 
               AtExtSrc eff_after_external23 core_at_external23 
               eff_after_external12 core_at_external12 HasTy1 HasTy2. 
-     subst. intros b Hb. rewrite REACHAX in Hb.
+     subst. intros b Hb. 
+    (* generalize (match_visible12 _ _ _ _ _ _ MC12); unfold REACH_closed; intros.
+     apply H. apply Hb.*)
+     
+      rewrite REACHAX in Hb.
       destruct Hb as [L HL].
       generalize dependent b.
       induction L; simpl; intros; inv HL.
-        apply H.
+      apply H.
       specialize (IHL _ H1); clear H1.
         apply orb_true_iff in IHL. apply orb_true_iff.
         destruct IHL.
@@ -561,8 +683,9 @@ Proof. (*follows structure of forward_simulations_trans.injinj*)
                 apply REACH_nil. apply H.
           right. eapply (inject_REACH_closed _ _ _ MemInjMu).
                 eapply REACH_cons; try eassumption.
-                apply REACH_nil. apply H.
-  remember (restrict_sm mu12 RESTR) as nmu12.
+                apply REACH_nil. apply H.*)
+  (*remember (restrict_sm mu12 RESTR) as nmu12.*)
+  remember mu12 as nmu12.
   assert (HmuNorm: mu = compose_sm nmu12 mu23).
      clear UnchLOOR13 UnchPrivSrc Mu'Hyp mu' frgnTgtHyp frgnTgt'
               frgnSrcHyp frgnSrc' FwdTgt FwdSrc RValInjNu' MemInjNu' 
@@ -571,7 +694,8 @@ Proof. (*follows structure of forward_simulations_trans.injinj*)
               AtExtSrc eff_after_external23 core_at_external23 
               eff_after_external12 core_at_external12 HasTy1 HasTy2. 
       subst nmu12 mu RESTR. unfold compose_sm; simpl.
-          rewrite restrict_sm_extern.
+          auto.
+          (*rewrite restrict_sm_extern.
           rewrite (restrict_sm_local' _ WDmu12).
           Focus 2. clear. intuition.
           unfold restrict_sm; simpl. 
@@ -590,7 +714,7 @@ Proof. (*follows structure of forward_simulations_trans.injinj*)
             remember (frgnBlocksSrc b) as q.
             destruct q; apply eq_sym in Heqq; simpl in *. reflexivity.
             remember (StructuredInjections.extern_of mu23 b2) as w.
-            destruct w; trivial. destruct p. rewrite <- Heqw. trivial.    
+            destruct w; trivial. destruct p. rewrite <- Heqw. trivial.  
          remember (locBlocksSrc b) as q. 
          destruct q; simpl; trivial.
          remember (frgnBlocksSrc b) as w.
@@ -598,7 +722,7 @@ Proof. (*follows structure of forward_simulations_trans.injinj*)
          remember (local_of b) as t.
          destruct t; simpl; trivial.
          destruct p; apply eq_sym in Heqt.
-         destruct (local_DomRng _ WDmu12 _ _ _ Heqt); simpl in *. congruence.  
+         destruct (local_DomRng _ WDmu12 _ _ _ Heqt); simpl in *. congruence.*)  
   clear MC12. 
   assert (WDnmu12:= match_sm_wd12 _ _ _ _ _ _ NormMC12).
   clear HMu.
@@ -606,7 +730,7 @@ Proof. (*follows structure of forward_simulations_trans.injinj*)
     eapply compose_sm_wd; try eassumption.
       subst. unfold restrict_sm, restrict; simpl. destruct mu12; simpl in *. apply GLUEINV.
       subst. unfold restrict_sm, restrict; simpl. destruct mu12; simpl in *. apply GLUEINV.
-  clear match_restrict12 match_visible12.
+  clear (*match_restrict12*) match_visible12.
   assert (mu12_valid:= match_sm_valid12 _ _ _ _ _ _ NormMC12).
   assert (mu23_valid:= match_sm_valid23 _ _ _ _ _ _ MC23).
   rename ret2 into ret3.  
@@ -633,13 +757,13 @@ Proof. (*follows structure of forward_simulations_trans.injinj*)
   assert (LeakedCompSrc: locBlocksSrc mu = locBlocksSrc nmu12 /\
                          extBlocksSrc mu = extBlocksSrc nmu12 /\
                         exportedSrc mu vals1 = exportedSrc nmu12 vals1). 
-     subst. clear - WDnmu12 WDmu. simpl.  
-        rewrite restrict_sm_locBlocksSrc.
+     subst. clear - WDnmu12 WDmu. simpl.
+        (*rewrite restrict_sm_locBlocksSrc.
         rewrite restrict_sm_extBlocksSrc.
+         rewrite restrict_sm_frgnBlocksSrc, restrict_sm_pubBlocksSrc.*)
         unfold exportedSrc. 
         rewrite sharedSrc_iff_frgnpub; trivial. simpl. 
         rewrite sharedSrc_iff_frgnpub; trivial.
-        rewrite restrict_sm_frgnBlocksSrc, restrict_sm_pubBlocksSrc.
         intuition.
   destruct LeakedCompSrc as [LSa [LSb LSc]]. 
     rewrite LSa, LSc in *. clear LSa LSb LSc.
@@ -661,12 +785,12 @@ Proof. (*follows structure of forward_simulations_trans.injinj*)
         subst.
         clear UnchLOOR13 UnchPrivSrc (*SEP*) INC MemInjMu ArgsInj12 MInj12.
               
-        rewrite restrict_sm_locBlocksTgt. (*sm_extern_normalize_exportedTgt; trivial.*)
+        (*rewrite restrict_sm_locBlocksTgt.*) (*sm_extern_normalize_exportedTgt; trivial.*)
            rewrite GlueA. intros b Hb. rewrite andb_true_iff in *.
         destruct Hb. split; trivial.
         eapply REACH_mono; try eassumption.
         unfold exportedTgt, exportedSrc, sharedTgt.
-        rewrite restrict_sm_frgnBlocksTgt, restrict_sm_pubBlocksTgt.
+        (*rewrite restrict_sm_frgnBlocksTgt, restrict_sm_pubBlocksTgt.*)
         rewrite sharedSrc_iff_frgnpub; trivial.
         intros. repeat rewrite orb_true_iff in *.
         intuition.
@@ -680,8 +804,8 @@ Proof. (*follows structure of forward_simulations_trans.injinj*)
             replace_locals_frgnBlocksSrc, replace_locals_frgnBlocksTgt,
             replace_locals_extBlocksSrc, replace_locals_extBlocksTgt.
      rewrite replace_locals_extern, replace_locals_local.
-     rewrite restrict_sm_extBlocksSrc, restrict_sm_locBlocksSrc,
-             restrict_sm_local, restrict_sm_extern.
+     (*rewrite restrict_sm_extBlocksSrc, restrict_sm_locBlocksSrc,
+             restrict_sm_local, restrict_sm_extern.*)
      f_equal. 
 
   clear NuHyp.
@@ -698,24 +822,32 @@ Proof. (*follows structure of forward_simulations_trans.injinj*)
               locBlocksSrc mu12 b || frgnBlocksSrc mu12 b
               || mapped (as_inj (compose_sm mu12 mu23)) b)))) vals1 vals2).
       clear - ArgsInj12 Heqnmu12 HeqRESTR.
-      rewrite restrict_sm_all. subst. rewrite restrict_sm_all in ArgsInj12.
-       rewrite restrict_nest in ArgsInj12.
+      rewrite restrict_sm_all. subst. (*rewrite restrict_sm_all in ArgsInj12.
+       rewrite restrict_nest in ArgsInj12. *)
        eapply val_list_inject_forall_inject.
        apply forall_inject_val_list_inject in ArgsInj12.
        eapply val_list_inject_incr; try eassumption.
        red; intros. destruct (restrictD_Some _ _ _ _ _ H); clear H.
-          unfold vis in H1. rewrite restrict_sm_locBlocksSrc, restrict_sm_frgnBlocksSrc in H1.
+          unfold vis in H1. (*rewrite restrict_sm_locBlocksSrc, restrict_sm_frgnBlocksSrc in H1.*)
           apply restrictI_Some; intuition.
-    intros. rewrite effect_properties.vis_restrict_sm in H.
+    (*intros. rewrite effect_properties.vis_restrict_sm in H.
       unfold vis in H. intuition. 
-  clear ArgsInj12.
+  clear ArgsInj12.*) 
+  assert (ArgsInj12': Forall2 (val_inject (as_inj nmu12) )
+                vals1 vals2).
+       move ArgsInj12 at bottom. 
+       clear - ArgsInj12.
+       induction ArgsInj12; econstructor.
+       eapply val_inject_restrictD; eauto.
+       assumption.
+
   assert (WDnu12: SM_wd (replace_locals nmu12 pubSrc' pubTgtMid')).
        subst.
        eapply replace_locals_wd; try eassumption.
          intros. apply andb_true_iff in H.
            destruct H as [locB R].
            destruct (REACH_local_REACH _ WDnmu12 _ _ _ _ 
-              MInj12 ArgsInj12R _ R locB) as [b2 [d1 [LOC12 R2]]].
+              MInj12 (*ArgsInj12R*) ArgsInj12' _ R locB) as [b2 [d1 [LOC12 R2]]].
            exists b2, d1; split; trivial.
            rewrite andb_true_iff, R2.
            split; trivial.
@@ -747,12 +879,21 @@ Proof. (*follows structure of forward_simulations_trans.injinj*)
      split. rewrite replace_locals_DOM. eapply mu23_valid.
      rewrite replace_locals_RNG. eapply mu23_valid.
   rewrite NU in INC(*, SEP*).
+  (*Discharge PURE HERE *)
+  assert (Pure: pure_comp_ext (replace_locals nmu12 pubSrc' pubTgtMid')
+    (replace_locals mu23 pubSrcMid' pubTgt') m1 m2).
+  { clear - pure.
+    unfold pure_comp_ext, pure_composition, pure_composition_locat, 
+    pure_composition_block, replace_locals, DomSrc, exportedSrc, sharedSrc, shared_of in *;
+      destruct nmu12, mu23; simpl in *. 
+    apply pure.
+  }
   destruct (EFFAX.effect_interp_II _ _ _ MinjNu12 _ FwdSrc
       _ _ MinjNu23 _ FwdTgt nu' WDnu' SMvalNu' MemInjNu'
-      INC (*SEP*) nu12_valid nu23_valid)
-     as [m2' [nu12' [nu23' [X [Incr12 [Incr23 [MInj12'
-        [Fwd2 [MInj23' (*[Sep12 [Sep23*) [nu12'valid
-        [nu23'valid [GLUEINV' [Norm' [UnchMidA UnchMidB]]]]]]]]]]]]]](*]]*); simpl in *.
+      INC Pure nu12_valid nu23_valid)
+     as [m2' [nu12' [nu23' [X [Incr12 [Incr23 [Pure' [MInj12'
+        [Fwd2 [MInj23' [nu12'valid
+        [nu23'valid [GLUEINV' [full' [UnchMidA UnchMidB ]]]]]]]]]]]]]]]; simpl in *.
     (*discharge the unchOn application conditions*)
        subst; apply UnchPrivSrc.
        subst. apply UnchLOOR13. 
@@ -763,13 +904,21 @@ Proof. (*follows structure of forward_simulations_trans.injinj*)
             replace_locals_frgnBlocksSrc, replace_locals_frgnBlocksTgt.
       destruct GLUEINV as [GLUEa [GLUEb [GLUEc GLUEd]]].
       repeat (split; trivial).
-      subst. rewrite restrict_sm_locBlocksTgt; trivial.
+      (*subst. rewrite restrict_sm_locBlocksTgt; trivial.
       subst. rewrite restrict_sm_extBlocksTgt; trivial.
-      subst. rewrite restrict_sm_frgnBlocksTgt; trivial.
-    (*discharge the Norm Hypothesis*)
-      rewrite Heqnmu12. do 2 rewrite replace_locals_extern.
-      rewrite restrict_sm_extern.
-      intros. destruct (restrictD_Some _ _ _ _ _ H) as [EX12 RR]; clear H.
+      subst. rewrite restrict_sm_frgnBlocksTgt; trivial.*)
+      (* NORM HERE*)
+      { unfold full_ext, full_comp, replace_locals; simpl.
+        subst nmu12.  
+        destruct mu12; destruct mu23; simpl.
+        exact full.
+        }
+      
+ 
+      (*discharge the Norm Hypothesis*)
+      (*rewrite Heqnmu12. do 2 rewrite replace_locals_extern.
+      (*rewrite restrict_sm_extern.*)
+      intros. (*destruct (restrictD_Some _ _ _ _ _ H) as [EX12 RR]; clear H.*)
       subst RESTR nmu12.
      clear UnchLOOR13 UnchPrivSrc Mu'Hyp mu' frgnTgtHyp frgnTgt'
               frgnSrcHyp frgnSrc' FwdTgt FwdSrc RValInjNu' MemInjNu' 
@@ -793,23 +942,23 @@ Proof. (*follows structure of forward_simulations_trans.injinj*)
           rewrite EX12 in E1. inv E1. rewrite E2. exists bb, dd2; trivial.
         rewrite compose_sm_local in LOC.
           destruct (compose_meminjD_Some _ _ _ _ _ LOC) as [bb2 [dd1 [dd2 [E1 [E2 D]]]]].
-          destruct (disjoint_extern_local _ WDmu12 b1); congruence.
+          destruct (disjoint_extern_local _ WDmu12 b1); congruence.*)
   assert (UnchMidC : Mem.unchanged_on (local_out_of_reach (replace_locals mu23 pubSrcMid' pubTgt') m2) m3 m3').
     clear - WDmu23 HeqpubTgtMid' HeqpubSrcMid' MinjNu12 UnchLOOR13 WDnu12 NU pubSrcHyp Heqnmu12 HeqRESTR GLUEINV.
     subst nmu12.
-    remember (replace_locals (restrict_sm mu12 RESTR) pubSrc' pubTgtMid') as kappa12.
+    remember (replace_locals (*restrict_sm mu12 RESTR*) mu12 pubSrc' pubTgtMid') as kappa12.
     remember (replace_locals mu23 pubSrcMid' pubTgt') as kappa23.
     assert (GluePubKappa : forall b : block,
           pubBlocksTgt kappa12 b = true -> pubBlocksSrc kappa23 b = true).
        clear UnchLOOR13 WDnu12 MinjNu12.
        subst kappa12 kappa23. rewrite replace_locals_pubBlocksSrc, replace_locals_pubBlocksTgt.
-       subst. rewrite restrict_sm_locBlocksTgt; intros; trivial.
+       subst. (*rewrite restrict_sm_locBlocksTgt;*) intros; trivial.
               apply andb_true_iff in H. destruct H.
               destruct GLUEINV as [Ga [Gb [Gc Gd]]]. rewrite Ga in H.
               rewrite H; simpl.
               eapply REACH_mono; try eassumption.
               unfold exportedTgt, exportedSrc, sharedTgt. rewrite sharedSrc_iff_frgnpub.
-              rewrite restrict_sm_frgnBlocksTgt, restrict_sm_pubBlocksTgt.
+              (*rewrite restrict_sm_frgnBlocksTgt, restrict_sm_pubBlocksTgt.*)
               intros. do 2 rewrite orb_true_iff in H1.
                 do 2 rewrite orb_true_iff. intuition.
            assumption.
@@ -853,6 +1002,7 @@ Proof. (*follows structure of forward_simulations_trans.injinj*)
           rewrite <- Arith.
           eapply MinjNu12. eapply pub_in_all; try eassumption. apply N.
         rewrite H in PubTgt2. discriminate.
+
   (*next, prepare for application of eff_after_external12*)
   destruct GLUEINV' as [WDnu12' [WDnu23' [GLUEa' [GLUEb' [GLUEc' GLUEd']]]]].
   assert (H: exists ret2, val_inject (as_inj nu12') ret1 ret2 /\ 
@@ -868,7 +1018,7 @@ Proof. (*follows structure of forward_simulations_trans.injinj*)
   subst. 
   assert (HasTy12: Val.has_type ret2 (proj_sig_res (AST.ef_sig e))). 
   { clear - HasTy2 RValInjNu23'. inv RValInjNu23'; auto. constructor. }
-  assert (LIES: globals_separate g2
+  (*assert (LIES: globals_separate g2
                            (replace_locals
                               (restrict_sm mu12
                                  (fun b : block =>
@@ -909,9 +1059,9 @@ Proof. (*follows structure of forward_simulations_trans.injinj*)
                                         || frgnBlocksSrc mu12 b0
                                         || mapped
                                              (as_inj (compose_sm mu12 mu23))
-                                             b0)) vals2) b)) nu12' ) by admit.
+                                             b0)) vals2) b)) nu12' ) by ad_it.*)
   specialize (eff_after_external12 nu12' ret1 
-     m1' ret2 m2' HasTy1 HasTy12 Incr12 LIES (*Sep12*) WDnu12' nu12'valid MInj12' RValInjNu12'
+     m1' ret2 m2' HasTy1 HasTy12 Incr12 (*LIES Sep12*) WDnu12' nu12'valid MInj12' RValInjNu12'
      FwdSrc Fwd2 (*RetType2*)).
 
   destruct (eff_after_external12 _ (eq_refl _) 
@@ -923,14 +1073,14 @@ Proof. (*follows structure of forward_simulations_trans.injinj*)
 
   (*next, apply eff_after_external23*)
   specialize (eff_after_external23 nu23').
-  assert (LIES3: globals_separate g3
+  (*assert (LIES3: globals_separate g3
     (replace_locals mu23
        (fun b : block =>
         locBlocksSrc mu23 b && REACH m2 (exportedSrc mu23 vals2) b)
        (fun b : block =>
-        locBlocksTgt mu23 b && REACH m3 (exportedTgt mu23 vals3) b)) nu23') by admit.
+        locBlocksTgt mu23 b && REACH m3 (exportedTgt mu23 vals3) b)) nu23') by ad_it.*)
   destruct (eff_after_external23 ret2 m2' 
-       ret3 m3' HasTy12 HasTy2 Incr23 LIES3 (*Sep23*) WDnu23' nu23'valid
+       ret3 m3' HasTy12 HasTy2 Incr23 (*LIES3 Sep23*) WDnu23' nu23'valid
        MInj23' RValInjNu23' Fwd2 FwdTgt (*RetTypeTgt*)
      _ (eq_refl _) _ (eq_refl _) _ (eq_refl _)) as
      [d23' [c22' [c3' [AftExt22 [AftExt3 MC23']]]]];
@@ -993,7 +1143,20 @@ Proof. (*follows structure of forward_simulations_trans.injinj*)
                             left. intuition.
                             right. intuition.
                assumption.
-   split; assumption. }
+   intuition.
+   (* PURE HERE *)
+   { clear - Pure'.
+     unfold pure_comp_ext, pure_composition, pure_composition_locat, 
+     pure_composition_block, replace_locals, DomSrc, exportedSrc, sharedSrc, shared_of in *;
+       destruct nu12', nu23'; simpl in *. 
+     apply Pure'.
+   }
+   (* NORM HERE*)
+   { unfold full_ext, full_comp, replace_externs; simpl.
+     destruct nu12'; destruct nu23'; simpl.
+     exact full'.
+   }
+}
 Qed.
 
 End Eff_sim_trans. 
