core/mem_interpolation_II3.v
@@ -1,0 +1,547 @@
+Require Import Events. (*is needed for some definitions (loc_unmapped etc*)
+Require Import Memory.
+Require Import Coqlib.
+Require Import Integers.
+Require Import Values.
+Require Import Maps.
+Require Import FiniteMaps.
+Require Import Axioms.
+
+Require Import mem_lemmas.
+Require Import mem_interpolation_defs.
+Require Import StructuredInjections.
+
+Require Import pure.
+Require Import full_composition.
+
+
+
+(***************************
+ * UNSTRUCTURED INJECTIONS *
+ ***************************)
+
+(*Shifts the image of an injection by n up
+ * The new target memory should be (size) large than
+ *)
+Definition shiftT (j: meminj) (n:block):meminj :=
+  fun b =>
+    match j b with
+        | Some (b2, d) => Some ((b2 + n)%positive, d)
+        | None => None
+    end.
+Infix ">>":= shiftT (at level 80, right associativity).
+
+(*Shifts the domain of an injection down by n
+ * The new target memory should be (size) large than
+ *)
+Definition shiftS (j: meminj) (n:block):meminj :=
+  fun b => match ( b ?= n)%positive with
+               | Gt => j (b - n)%positive
+               | _ => None
+           end.
+Infix "<<":= shiftS (at level 80, right associativity).
+
+(* fID satisfies (fID .*. f) = f and it's pure *)  
+Definition filter_id (j:meminj): meminj:=
+  fun b =>
+    match j b with
+        | Some _ => Some (b, 0)
+        | None => None
+    end.
+
+(* size is the size of the memory being mapped
+ * The new target memory should be (size) large than 
+ * the original memory.
+ *)
+Definition add_inj (j k: meminj): meminj := 
+  fun b =>
+    match j b with
+      | Some p => Some p
+      | None => k b
+    end.
+
+Infix "(+)":= add_inj (at level 90, right associativity).
+
+(* New definition for mkInjection
+ * Assumes the new middle memory is the addition of m1 and m2
+ * So everything mapped by j * k, is mapped identically
+ * And everything else, mapped only by l, passes through the 
+ * extra memory space added in m2 (of size m1).
+ *)
+Definition mkInjections (sizeM2:block)(j k l: meminj) 
+                     :  meminj * meminj := 
+   (j (+) (filter_id l >> sizeM2),
+    k (+) ( l << sizeM2)).
+
+(* Legacy: mkInjection that matches the type of the old version *)
+Definition mkInjections' (m1 m1' m2 :mem)(j k l: meminj) 
+                     :  meminj * meminj * block * block := 
+  let n1 := Mem.nextblock m1' in
+  let n2 := Mem.nextblock m2 in
+  match mkInjections n2 j k l with
+      | (j', k') => (j', k', n1, (n2 + n1)%positive)
+                      end.
+
+
+(**************************
+ * mkInjection Properties *
+ **************************)
+
+Lemma pos_be_pos: forall a b, (a + b ?= b = Gt)%positive.
+  intros. apply Pos.gt_iff_add. exists a. apply Pos.add_comm.
+Qed.
+
+Lemma MKIcomposition:
+  forall j k l sizeM2,
+    full_comp j k ->
+    inject_incr (compose_meminj j k) l ->
+    (forall b p, k b = Some p -> (b < sizeM2)%positive) ->
+    forall  j' k',
+      mkInjections sizeM2 j k l = (j', k') ->
+      l = compose_meminj j' k'.
+  unfold mkInjections; intros j k l ? full incr valid j' k' mk. inversion mk.
+  unfold add_inj, shiftT, shiftS, compose_meminj, filter_id.
+  extensionality b.
+  destruct (j b) eqn:jb. destruct p.
+  destruct (k b0) eqn:kb. destruct p.
+  + apply incr. unfold compose_meminj; rewrite jb; rewrite kb; trivial.
+  + apply full in jb. destruct jb as [b2 [d' kb0]]. rewrite kb0 in kb; inversion kb.
+  + destruct (l b) eqn:lb; trivial.
+    destruct (k (b + sizeM2)%positive) eqn: ksmthng. 
+    - apply valid in ksmthng.
+      clear - ksmthng; contradict ksmthng. rewrite Pos.add_comm; apply Pos.lt_not_add_l.
+    - rewrite (Pos.add_sub), lb. rewrite pos_be_pos; destruct p; auto.
+Qed.
+
+Lemma  MKI_incr12:
+  forall j k l sizeM2,
+    forall j' k',
+      (j', k') = mkInjections sizeM2 j k l ->
+   inject_incr j j'.
+  intros j k l sizeM2 j' k' MKI; inversion MKI.
+  unfold inject_incr, add_inj, shiftT. intros b b' d H; rewrite H; auto.
+Qed.
+
+Lemma  MKI_incr23:
+  forall j k l sizeM2,
+    forall j' k',
+      (j', k') = mkInjections sizeM2 j k l ->
+   inject_incr k k'.
+  intros j k l sizeM2 j' k' MKI; inversion MKI.
+  unfold inject_incr, add_inj, shiftT. intros b b' d H; rewrite H; auto.
+Qed.
+
+Lemma MKI_norm:
+  forall j k l sizeM2,
+    full_comp j k ->
+    (forall b p, k b = Some p -> (b < sizeM2)%positive) ->
+    forall j' k',
+      (j', k') = mkInjections sizeM2 j k l ->
+      full_comp j' k'.
+  unfold full_comp. intros j k l sizeM2 full valid j' k' MKI b0 b1 delta1 mapj.
+  inversion MKI.
+  assert (map:= mapj); clear mapj.
+  rewrite H0 in map; unfold add_inj in map.
+  destruct (j b0) eqn:jb0.
+  + destruct p; inversion map.
+    apply full in jb0; destruct jb0 as [b2 [delta2 kb1]].
+    exists b2, delta2.
+    unfold add_inj, shiftT.
+    subst b; rewrite kb1; auto.
+  + unfold shiftT in map.
+    destruct (filter_id l b0) eqn:filter_l; try solve[inversion map].
+    destruct p; inversion map.
+    unfold add_inj, shiftS.
+    destruct (k (b + sizeM2)%positive) eqn:mapk.
+    - apply valid in mapk.
+      contradict mapk. rewrite Pos.add_comm; apply Pos.lt_not_add_l.
+    - unfold filter_id in filter_l. destruct (l b0) eqn:lb0; try solve [inversion filter_l].
+      destruct p. rewrite Pos.add_sub. inversion filter_l. subst b0.
+      rewrite pos_be_pos; exists b2, z0; trivial.
+Qed.
+
+Lemma destruct_inj12:
+  forall j k l sizeM2,
+    forall j' k',
+      (j', k') = mkInjections sizeM2 j k l ->
+      forall (b1 b2 : block) (d1 : Z),
+        j' b1 = Some (b2, d1) ->
+        j b1 = Some (b2, d1) \/
+        (exists (b3 : block) (d : Z), l b1 = Some (b3, d)).
+  intros.
+  inversion H. subst j' k'.
+  unfold add_inj, shiftT in H0.
+  destruct (j b1) eqn:jb1.
+  + left. destruct p; inversion H0; auto.
+  + right. destruct (filter_id l b1) eqn:filtl; try solve [inversion H0].
+    destruct p. unfold filter_id in filtl.
+    destruct (l b1); try solve[ inversion filtl].
+    destruct p as [b3 d]; exists b3, d; auto.
+    
+Qed.
+
+Lemma destruct_inj23:
+  forall j k l sizeM2,
+    forall j' k',
+      (j', k') = mkInjections sizeM2 j k l ->
+      forall (b2 b3 : block) (d2 : Z),
+        k' b2 = Some (b3, d2) ->
+        k b2 = Some (b3, d2) \/
+        (exists (b1 : block), l b1 = Some (b3, d2)).
+  intros.
+  inversion H. subst j' k'.
+  unfold add_inj, shiftS in H0.
+  destruct (k b2) eqn:jb2.
+  + left. destruct p; inversion H0; auto.
+  + right. destruct ((b2 ?= sizeM2)%positive); try solve[inversion H0].
+    exists (b2 - sizeM2)%positive; trivial.
+Qed.
+
+(* Legacy: The following lemmas mathc some old lemmas. Probably useless now. *)
+Definition removeUndefs (j l j':meminj):meminj := 
+   fun b => match j b with 
+              None => match l b with 
+                         None => None | Some (b1,delta1) => j' b 
+                      end
+            | Some p => Some p
+            end.
+
+Lemma Undefs_removed:
+  forall j k l sizeM2 j' k', 
+    mkInjections sizeM2 j k l = (j', k') ->
+    j' = removeUndefs j l j'.
+  unfold mkInjections; intros. inversion H.
+  unfold add_inj, shiftT, shiftS, removeUndefs.
+  extensionality b. 
+  destruct (j b) eqn:jb; trivial.
+  unfold filter_id.
+  destruct (l b) eqn:lb; trivial.
+  destruct p; trivial.
+Qed.
+
+Lemma RU_composememinj: 
+  forall j k l sizeM2,
+    full_comp j k ->
+    inject_incr (compose_meminj j k) l ->
+    (forall b p, k b = Some p -> (b < sizeM2)%positive) ->
+    forall  j' k',
+    mkInjections sizeM2 j k l = (j', k') ->
+    l = compose_meminj (removeUndefs j l j') k'.
+  intros. erewrite <- Undefs_removed; eauto.
+  eapply MKIcomposition; eauto.
+Qed.
+
+Lemma RU_composememinj': forall m1 m1' m2 j k l j' k' n1' n2' 
+       (HI: mkInjections' m1 m1' m2 j k l = (j',k',n1',n2'))
+       (InjIncr: inject_incr (compose_meminj j k) l)
+       (m3: mem)
+       (InjSep: full_comp j k)
+       (VBj1: forall b1 b2 ofs2, j b1 = Some(b2,ofs2) -> Mem.valid_block m1 b1)
+       (VBj2: forall b1 b2 ofs2, j b1 = Some(b2,ofs2) -> Mem.valid_block m2 b2)
+       (VBk2: forall b1 b2 ofs2, k b1 = Some(b2,ofs2) -> Mem.valid_block m2 b1)
+       (VBL1': forall b1 b3 ofs3, l b1 = Some (b3, ofs3) -> (b1 < n1')%positive),
+      l = compose_meminj (removeUndefs j l j') k'.
+ intros. 
+ apply (RU_composememinj j k l (Mem.nextblock m2) InjSep); eauto. 
+ intros; destruct p; eapply VBk2; eauto.
+ unfold mkInjections' in HI. destruct (mkInjections (Mem.nextblock m2) j k l); inversion HI; auto.
+Qed.
+
+
+
+
+
+
+
+
+(*************************
+ * STRUCTURED INJECTIONS *
+ *************************)
+
+Definition buni (bset1 bset2: block -> bool): block -> bool :=
+  fun b => bset1 b || bset2 b.
+
+Definition bshift (bset : block -> bool) (num: block): block -> bool :=
+  fun b => match (b ?= num)%positive with
+             | Lt => false
+             | _ => bset (b-num)%positive 
+           end.
+
+Definition bconcat (bset1 bset2: block -> bool) (num: block) : block -> bool :=
+  buni bset1 (bshift bset2 num).
+
+Definition change_ext (mu: SM_Injection) extS extT (ext_inj: meminj): SM_Injection :=
+  match mu with
+    | {| locBlocksSrc := locBSrc;
+         locBlocksTgt := locBTgt;
+         pubBlocksSrc := pubBSrc;
+         pubBlocksTgt := pubBTgt;
+         local_of := local;
+         extBlocksSrc := extBSrc;
+         extBlocksTgt := extBTgt;
+         frgnBlocksSrc := fSrc;
+         frgnBlocksTgt := fTgt;
+         extern_of := extern |} =>
+      Build_SM_Injection
+       locBSrc
+       locBTgt
+       pubBSrc
+       pubBTgt
+       local
+       extS (* This changes *)
+       extT (* This changes *)
+       fSrc
+       fTgt
+       ext_inj (* This changes *)
+    end.
+
+(*************************
+ * STRUCTURED Properties *
+ *************************)
+
+Lemma bconcat_larger1: 
+  forall set1 set2 num b,
+    set1 b = true -> 
+    bconcat set1 set2 num b = true.
+  intros s1 s2 n b H; unfold bconcat, buni, bshift; rewrite H; auto.
+Qed.
+Lemma bconcat_larger2: 
+  forall set1 set2 num b,
+    set2 b = true -> 
+    bconcat set1 set2 num (b + num)%positive = true.
+  intros s1 s2 n b H; unfold bconcat, buni, bshift.
+  rewrite pos_be_pos; rewrite Pos.add_sub, H; apply orb_true_r.
+Qed.
+
+
+
+Lemma change_ext_partial_wd: 
+  forall mu,
+    SM_wd mu ->
+    forall mu' extS extT j,
+      mu' = change_ext mu extS extT j ->
+      (forall (b1 b2 : block) (z : Z),
+                   local_of mu' b1 = Some (b2, z) ->
+                   locBlocksSrc mu' b1 = true /\ locBlocksTgt mu' b2 = true) /\
+      (forall b1 : block,
+               pubBlocksSrc mu' b1 = true ->
+               exists (b2 : block) (z : Z),
+                 local_of mu' b1 = Some (b2, z) /\ pubBlocksTgt mu' b2 = true) /\
+      (forall b : block,
+                        pubBlocksTgt mu' b = true -> locBlocksTgt mu' b = true).
+  intros ? SMWD ? ? ? ? ? . subst mu'. destruct SMWD.
+  unfold change_ext; destruct mu; simpl in *; intuition.
+Qed.
+
+
+Lemma MKI_wd12:
+  forall mu12 j k l sizeM2,
+    SM_wd mu12 ->
+    j = extern_of mu12 ->
+    forall j' k',
+      (j', k') = mkInjections sizeM2 j k l ->
+      forall extS extT
+         (disjoint_extern_local_Src : 
+            forall b : block, locBlocksSrc mu12 b = false \/extS b = false)
+         (disjoint_extern_local_Tgt : 
+            forall b : block, locBlocksTgt mu12 b = false \/ extT b = false)
+         (extern_DomRng : forall (b1 b2 : block) (z : Z),
+                  j' b1 = Some (b2, z) -> extS b1 = true /\ extT b2 = true)
+         (frgnBlocksExternTgt : forall b : block,
+                        frgnBlocksTgt mu12 b = true -> extT b = true),
+   SM_wd (change_ext mu12 extS extT j').
+  intros mu12 j k l sizeM2 SMWD jID j' k' MKI extS extT.
+  intros disjoint_extern_local_Src
+         disjoint_extern_local_Tgt
+         extern_DomRng
+         frgnBlocksExternTgt.
+  unfold change_ext; destruct mu12; simpl in *.
+  destruct SMWD; constructor; simpl in *; auto.
+  (* remains to prove frgnSrcAx *)
+  { intros.
+    apply frgnSrcAx in H.
+    destruct H as [b2 [z2 [extof frgnB]]].
+    exists b2, z2.
+    split; auto.
+    inversion MKI; inversion jID.
+    unfold add_inj. rewrite extof; auto. 
+  }
+Qed.
+
+Lemma MKI_wd23:
+  forall mu23 j k l sizeM2,
+    SM_wd mu23 ->
+    k = extern_of mu23 ->
+    forall j' k',
+      (j', k') = mkInjections sizeM2 j k l ->
+      forall extS extT
+         (disjoint_extern_local_Src : 
+            forall b : block, locBlocksSrc mu23 b = false \/extS b = false)
+         (disjoint_extern_local_Tgt : 
+            forall b : block, locBlocksTgt mu23 b = false \/ extT b = false)
+         (extern_DomRng : forall (b1 b2 : block) (z : Z),
+                  k' b1 = Some (b2, z) -> extS b1 = true /\ extT b2 = true)
+         (frgnBlocksExternTgt : forall b : block,
+                        frgnBlocksTgt mu23 b = true -> extT b = true),
+   SM_wd (change_ext mu23 extS extT k').
+  intros mu23 j k l sizeM2 SMWD jID j' k' MKI extS extT.
+  intros disjoint_extern_local_Src
+         disjoint_extern_local_Tgt
+         extern_DomRng
+         frgnBlocksExternTgt.
+  unfold change_ext; destruct mu23; simpl in *.
+  destruct SMWD; constructor; simpl in *; auto.
+  (* remains to prove frgnSrcAx *)
+  { intros.
+    apply frgnSrcAx in H.
+    destruct H as [b2 [z2 [extof frgnB]]].
+    exists b2, z2.
+    split; auto.
+    inversion MKI; inversion jID.
+    unfold add_inj. rewrite extof; auto. 
+  }
+Qed.
+
+
+(*I don't know why the following are needed.*)
+Lemma destruct_sminj12:
+  forall nu12 j,
+    SM_wd nu12 ->
+    j = extern_of nu12 ->
+    forall nu' l,
+      l = extern_of nu' ->
+      forall k sizeM2 j' k',
+        (j', k') = mkInjections sizeM2 j k l ->
+        forall extS extT,
+        forall (b1 b2 : block) (d1 : Z),
+          as_inj (change_ext nu12 extS extT j') b1 = Some (b2, d1) ->
+          as_inj nu12 b1 = Some (b2, d1) \/
+          (exists (b3 : block) (d : Z), as_inj nu' b1 = Some (b3, d)).
+  unfold as_inj, join, change_ext;
+  intros nu12 j SMWD jID nu' l lID k sizeM2 j' k' MKI extT extS b1 b2 d1; 
+  destruct nu12; simpl in *.
+  destruct (j' b1)  eqn:jb1.
+  + destruct p. inversion MKI. 
+    eapply destruct_inj12 in jb1; eauto; destruct jb1.
+    - left. rewrite <- jID; rewrite H.
+      inversion H2; subst; auto.
+    - right. destruct H as [b3 [d3 lb1]]; rewrite <- lID; rewrite lb1.
+      exists b3, d3; auto.
+  + intros. apply disjoint_extern_local in SMWD.
+    simpl in SMWD; destruct (SMWD b1) as [extNone | locNone].
+    - left; rewrite extNone; exact H.
+    - rewrite locNone in H; inversion H.
+Qed.
+
+Lemma destruct_sminj23:
+  forall nu23 k,
+    SM_wd nu23 ->
+    k = extern_of nu23 ->
+    forall nu' l,
+      l = extern_of nu' ->
+      forall j sizeM2 j' k',
+        (j', k') = mkInjections sizeM2 j k l ->
+        forall extS extT,
+        forall (b2 b3 : block) (d2 : Z),
+          as_inj (change_ext nu23 extS extT k') b2 = Some (b3, d2) ->
+          as_inj nu23 b2 = Some (b3, d2) \/
+          (exists (b1 : block), as_inj nu' b1 = Some (b3, d2)).
+  unfold as_inj, join, change_ext;
+  intros nu23 j SMWD jID nu' l lID k sizeM2 j' k' MKI extT extS b2 b3 d2; 
+  destruct nu23; simpl in *.
+  destruct (k' b2)  eqn:kb2.
+  + destruct p. inversion MKI. 
+    eapply destruct_inj23 in kb2; eauto; destruct kb2.
+    - left. rewrite <- jID; rewrite H.
+      inversion H2; subst; auto.
+    - right. destruct H as [b1 lb1]; rewrite <- lID. 
+      exists b1; rewrite lb1; trivial.
+  + intros. apply disjoint_extern_local in SMWD.
+    simpl in SMWD; destruct (SMWD b2) as [extNone | locNone].
+    - left; rewrite extNone; exact H.
+    - rewrite locNone in H; inversion H.
+Qed.
+
+(*************************
+ *         MEMORY        *
+ *************************)
+Parameter mem_add: mem -> mem -> mem.
+
+Definition mem_add_cont (m1 m2:mem):=
+  fun (b: block)=>
+    let n1 := (Mem.nextblock m1) in
+    match (b ?= n1)%positive with
+        | Lt => (Mem.mem_contents m1) !! b
+        | _ => (Mem.mem_contents m1) !! (b - n1)
+    end.
+Definition mem_add_acc (m1 m2:mem):=
+  fun (b: block)=>
+    let n1 := (Mem.nextblock m1) in
+    match (b ?= n1)%positive with
+        | Lt => (Mem.mem_access m1) !! b
+        | _ => (Mem.mem_access m1) !! (b - n1)
+    end.
+Definition mem_add_nb (m1 m2:mem):=
+  let n1 := Mem.nextblock m1 in
+  let n2 := Mem.nextblock m2 in
+  (n1 + n2)%positive. 
+
+Axiom mem_add_ax: forall (m1 m2 m3: mem), 
+                    m3 = mem_add m1 m2 ->
+                    (forall b, (Mem.mem_contents m3) !! b = mem_add_cont m1 m2 b) /\
+                    (forall b, (Mem.mem_access m3) !! b  = mem_add_acc m1 m2 b) /\
+                    (Mem.nextblock m3 = mem_add_nb m1 m2).
+
+Lemma mem_add_contx: forall (m1 m2: mem),
+                    (forall b, (Mem.mem_contents (mem_add m1 m2)) !! b = mem_add_cont m1 m2 b).
+  intros; remember (mem_add m1 m2) as m3; apply mem_add_ax; auto.
+Qed.
+
+Lemma mem_add_accx: forall (m1 m2: mem),
+                    (forall b, (Mem.mem_access (mem_add m1 m2)) !! b = mem_add_acc m1 m2 b).
+  intros; remember (mem_add m1 m2) as m3; apply mem_add_ax; auto.
+Qed.
+
+Lemma mem_add_nbx: forall (m1 m2: mem),
+                    (Mem.nextblock (mem_add m1 m2)) = mem_add_nb m1 m2.
+  intros; remember (mem_add m1 m2) as m3; apply mem_add_ax; auto.
+Qed.
+
+(*************************
+ *    MEMORY PROPRTIES   *
+ *************************)
+
+Lemma mem_add_forward: forall m1' m2,
+  mem_forward m2 (mem_add m2 m1').
+  unfold mem_forward. intros m1' m2 b bval_m2.
+  split.
+  + unfold Mem.valid_block in *.
+    rewrite mem_add_nbx.
+    unfold mem_add_nb.
+    apply (Plt_trans _ _ _ bval_m2). 
+    apply Pos.lt_iff_add; exists ( Mem.nextblock m1'); auto.
+  + unfold Mem.valid_block, Plt, Pos.lt in bval_m2.
+    unfold Mem.perm. rewrite mem_add_accx; unfold mem_add_acc.
+    rewrite bval_m2; auto.
+Qed.
+
+Lemma mem_add_unchanged: 
+  forall m1' m2,
+    let in_m2 := fun b z => Plt b (Mem.nextblock m2) in
+    Mem.unchanged_on in_m2 m2 (mem_add m2 m1').
+  intros; constructor; intros.
+  unfold in_m2 in H. 
+  + unfold Mem.perm. rewrite mem_add_accx; unfold mem_add_acc. 
+    rewrite H; split; trivial.
+  + unfold Mem.perm. rewrite mem_add_contx; unfold mem_add_cont. 
+    rewrite H; split; trivial.
+Qed.
+
+
+(*mem_unchanged_on_sub*)
+  
+
+(*Lemma MKI_meminj12:
+  forall j k l m1' m2,
+    Mem.inject j 
+    forall *)
