core/no_junk.v
@@ -1,0 +1,174 @@
+
+
+Require Import Memory.
+Require Import Maps.
+Require Import Coqlib.
+Require Import Values.
+
+Require Import StructuredInjections.
+Require Import effect_simulations_lemmas.
+Require Import mem_interpolation_defs.
+ 
+Load Santiago_tactics.
+
+Local Notation "a # b" := (PMap.get b a) (at level 1).
+Local Notation "a ## b" := (ZMap.get b a) (at level 1).
+
+Definition junk_inv_r mu m1 m2 m2' :=
+  (forall (b2: block) delta ofs,
+    locBlocksTgt mu b2 = true  ->
+    (Mem.perm m2 b2 (delta + ofs) = Mem.perm m2' b2 (delta + ofs) ) /\
+    ((Mem.mem_contents m2) # b2 ## (delta + ofs) = (Mem.mem_contents m2') # b2 ## (delta + ofs) )) /\
+  (forall (b1 b2: block) delta ofs,
+    extern_of mu b1 = Some( b2, delta) ->
+    Mem.perm m1 b1 ofs Max Nonempty -> 
+    (Mem.perm m2 b2 (delta + ofs) = Mem.perm m2' b2 (delta + ofs) ) /\
+    ((Mem.mem_contents m2) # b2 ## (delta + ofs) = (Mem.mem_contents m2') # b2 ## (delta + ofs) )).
+
+Lemma junk_inv_r_refl: forall mu m1 m2, junk_inv_r mu m1 m2 m2.
+  unfold junk_inv_r; intros; auto.
+Qed.
+
+Lemma junk_inv_r_sym: forall mu m1 m2 m2', junk_inv_r mu m1 m2 m2' -> junk_inv_r mu m1 m2' m2.
+  
+  unfold junk_inv_r; intros mu m1 m2 m2' H; split; intros;
+  destruct H as [loc ext].
+  split ; symmetry; specialize (loc b2 delta ofs H0); destruct loc; assumption.
+  split ; symmetry; specialize (ext b1 b2 delta ofs H0 H1); destruct ext; assumption.
+Qed.
+
+Lemma junk_inv_r_trans: forall mu m1 m2 m2' m2'', junk_inv_r mu m1 m2 m2' -> junk_inv_r mu m1 m2' m2'' -> junk_inv_r mu m1 m2 m2''.
+  unfold junk_inv_r; intros mu m1 m2 m2' m2'' H1 H2; split; intros;
+  destruct H1 as [loc1 ext1];  destruct H2 as [loc2 ext2].
+  specialize (loc1 b2 delta ofs H); destruct loc1;
+  specialize (loc2 b2 delta ofs H); destruct loc2; split; rewriter; auto.
+  specialize (ext1 b1 b2 delta ofs H H0); destruct ext1;
+  specialize (ext2 b1 b2 delta ofs H H0); destruct ext2;
+  split; rewriter; eauto.
+Qed.
+
+Definition junk_inv_l mu m m' :=
+  forall (b1 b1': block) delta ofs,
+    (as_inj mu) b1 = Some (b1', delta)  ->
+    (Mem.perm m b1 (ofs) = Mem.perm m' b1 (ofs) ) /\
+    ((Mem.mem_contents m) # b1 ## (ofs) = (Mem.mem_contents m') # b1 ## (ofs) ).
+
+Lemma junk_inv_l_refl: forall mu m, junk_inv_l mu m m.
+  unfold junk_inv_l; intros; auto.
+Qed.
+
+Lemma junk_inv_l_sym: forall mu m m', junk_inv_l mu m m' -> junk_inv_l mu m' m.
+  unfold junk_inv_l; intros mu m m' H; intros;
+  split ; symmetry; specialize (H b1 b1' delta ofs H0); destruct H; assumption.
+Qed.
+
+Lemma junk_inv_l_trans: forall mu m m' m'', junk_inv_l mu m m' -> junk_inv_l mu m' m'' -> junk_inv_l mu m m''.
+  unfold junk_inv_l; intros mu m m' m'' H1 H2; split; intros;
+  specialize (H1 b1 b1' delta ofs H); destruct H1;
+  specialize (H2 b1 b1' delta ofs H); destruct H2; rewriter; auto.
+Qed.
+
+
+(** *No Junk *)
+Definition no_junk_r (mu12:SM_Injection)(m1 m2: mem): Prop :=
+  forall b2 ofs, 
+            Mem.perm m2 b2 ofs Max Nonempty ->
+            extBlocksTgt mu12 b2 = true ->
+            exists b1 delta12,
+            (extern_of mu12) b1 = Some (b2, delta12 ) /\
+            Mem.perm m1 b1 (ofs - delta12) Max Nonempty.
+
+
+(** *Transitivity when the middle memory doesn't change*)
+Lemma no_junk_r_trans: forall mu mu12 mu23,
+                       SM_wd mu12 ->
+                       SM_wd mu23 ->
+                       mu = compose_sm mu12 mu23 ->
+                       extBlocksTgt mu12 = extBlocksSrc mu23 ->
+                       forall m1 m2 m3 m3',
+                         junk_inv_r mu m1 m3 m3' ->
+                         no_junk_r mu12 m1 m2 ->
+                         junk_inv_r mu23 m2 m3 m3'.
+  unfold junk_inv_r;
+  intros mu mu12 mu23 WD12 WD23 comp extB m1 m2 m3 m3' JINV NJNK.
+  unfold no_junk_r in NJNK.
+  
+  split.
+  {(*locals*)
+    intros b2 delta ofs loc_of.
+    destruct JINV as [JINVloc JINVext].
+    eapply JINVloc; eauto.
+    rewrite comp; unfold compose_sm, compose_meminj; simpl; assumption.
+  }
+  { (*externals*) intros b1 b2 delta ofs ext_of perm.
+  destruct (NJNK b1 ofs) as [b0 [delta12 [ext_of' perm']]]; eauto.
+  rewrite extB; apply WD23 in ext_of; destruct ext_of; assumption.
+  
+  assert (arith: delta + ofs = (delta12 + delta) + (ofs - delta12)) by xomega;
+    rewrite arith.
+  eapply JINV; eauto.
+  rewrite comp; unfold compose_sm, compose_meminj; simpl.
+  erewrite ext_of', ext_of; reflexivity. 
+  }
+Qed.
+
+(** *Clean memory: a mem with no junk*)
+
+Definition is_not_mapped mu m1 b' ofs :=
+  match source (as_inj mu) m1 b' ofs with
+      Some _ => false
+    | None => true
+  end.
+
+(* checks if a location is external and NOT  mapped *)
+Definition is_junk m mu b' ofs:=
+  (extBlocksTgt mu b') && (is_not_mapped mu m b' ofs).
+                       
+
+(*Removes all junk from one block in m2. i.e. Removes permition to locations that are not mapped from m1 *)
+Definition clean_block_access (mu: SM_Injection) m1 b' (access2: Z -> perm_kind -> option permission): Z -> perm_kind -> option permission :=
+  fun ofs pk =>
+    match access2 ofs pk with
+        | None => None
+        | Some perm => if is_junk m1 mu b' ofs then None else Some perm 
+    end.
+
+(*
+Definition filter2 (A: Type) (pred: elt -> bool) (m: t A) {struct m} : t A :=
+    match m with
+    | Leaf => Leaf
+    | Node l o r =>
+        let o' := match o with None => None | Some x => if pred x then o else None end in
+        Node' (filter1 pred l) o' (filter1 pred r)
+    end.
+
+Definition clean_block_content mu m1 b' (content2: ZMap.t memval):=
+  map1 (fun ofs => if is_junk m1 mu b' ofs then None else )
+
+  *)
+
+
+
+Definition clean (mu: SM_Injection) (m1 m2:mem) : mem.
+  Admitted.
+
+Lemma clean_junk_inv_r: forall mu m1 m2, junk_inv_r mu m1 m2 (clean mu m1 m2).
+Admitted.
+
+Lemma clean_junk_inv_l: forall mu m1 m2, junk_inv_l mu m2 (clean mu m1 m2).
+Admitted.
+
+Lemma clean_no_junk: forall mu m1 m2, no_junk_r mu m1 (clean mu m1 m2).
+Admitted.
+
+Theorem ex_clean_mem: forall mu m1 m2, exists m2', junk_inv_r mu m1 m2 m2' /\ no_junk_r mu m1 m2'.
+  intros.
+  exists (clean mu m1 m2).
+  split; [apply clean_junk_inv_r | apply clean_no_junk].
+Qed.
+
+Theorem ex_clean_mem_mid: forall mu12 m1 m2, exists m2', junk_inv_r mu12 m1 m2 m2' /\ no_junk_r mu12 m1 m2'.
+  intros.
+  exists (clean mu12 m1 m2).
+  split; [apply clean_junk_inv_r | apply clean_no_junk].
+Qed.
