core/pure.v
@@ -1,0 +1,59 @@
+Require Import Events.
+Require Import Memory.
+Require Import Coqlib.
+Require Import Values.
+Require Import Maps.
+Require Import Integers.
+Require Import AST.
+Require Import Globalenvs.
+Require Import Axioms.
+Require Import Memory.
+Require Import StructuredInjections.
+Require Import reach.
+
+Definition valid_location m b ofs:= Mem.perm m b ofs Max Nonempty.
+
+(*Parameter pure_composition: SM_Injection -> SM_Injection -> mem -> mem -> mem -> Prop.*)
+
+
+
+Definition pure_composition_locat (j12 j23:meminj) m1 m2:=
+  forall b2 b3 ofs23 delta,
+         j23 b2 = Some (b3, ofs23) ->
+         valid_location m2 b2 delta ->
+         exists b1 ofs12,
+           j12 b1 = Some (b2, ofs12) /\
+           valid_location m1 b1 (delta - ofs12).
+Definition pure_composition_block (j12 j23: meminj):=
+  forall b2 b3 ofs23,
+         j23 b2 = Some (b3, ofs23) ->
+         exists b1 ofs12,
+           j12 b1 = Some (b2, ofs12).
+
+Definition pure_composition j12 j23 m1 m2 :=
+  pure_composition_locat j12 j23 m1 m2 /\ pure_composition_block j12 j23.
+
+Definition pure_comp_ext mu12 mu23 m1 m2 := pure_composition (extern_of mu12) (extern_of mu23) m1 m2 .
+
+(*Making stuff up here: *)
+(*Lemma pure_frgn: forall mu12 mu23 m1 m2 m3, 
+                   SM_wd mu23 ->
+                   pure_composition mu12 mu23 m1 m2 m3 ->
+                   forall b',
+                   frgnBlocksSrc mu23 b' = true ->
+                   exists b ofs, 
+                     extern_of mu12 b = Some (b', ofs) /\
+                     frgnBlocksSrc mu12 b = true.
+intros ? ? ? ? ? SMWD pure b' frgn.
+apply pureAX in pure; destruct pure as [pure_loc pure_block].
+unfold pure_composition_block in pure_block.
+assert (frgn':= frgn).
+apply SMWD in frgn; destruct frgn as [b2 [ofs23 [extof frgn]]].
+destruct (pure_block b' b2 ofs23 extof frgn') as [b1 [ofs12 extof']].
+exists b1, ofs12.
+split; auto.
+
+assert (HH:as_inj mu23 b' = Some (b2, ofs23)) by admit. (* follows from extof and SMWD*)
+
+
+Admitted.*)
